

Example 3. If $u = \frac{x}{y-z}$, $v = \frac{y}{z-x}$, $w = \frac{z}{x-y}$, show that $\frac{\partial(u, v, w)}{\partial(x, y, z)} = 0$.

Sol. Here

$$u = \frac{x}{y-z}, v = \frac{y}{z-x}, w = \frac{z}{x-y}$$

\Rightarrow

$$\log u = \log x - \log(y-z) \quad \dots(1)$$

$$\log v = \log y - \log(z-x) \quad \dots(2)$$

$$\log w = \log z - \log(x-y) \quad \dots(3)$$

Differentiating (1) partially w.r.t. x

$$\frac{1}{u} \cdot \frac{\partial u}{\partial x} = \frac{1}{x} \Rightarrow \frac{\partial u}{\partial x} = \frac{u}{x}$$

Differentiating (1) partially w.r.t. y

$$\frac{1}{u} \cdot \frac{\partial u}{\partial y} = -\frac{1}{y-z} \Rightarrow \frac{\partial u}{\partial y} = \frac{-u}{y-z}$$

Differentiating (1) partially w.r.t. z

$$\frac{1}{u} \cdot \frac{\partial u}{\partial z} = -\frac{1}{y-z} (-1) \Rightarrow \frac{\partial u}{\partial z} = \frac{u}{y-z}$$

Similarly from (2) and (3), we have

$$\frac{\partial v}{\partial x} = \frac{v}{z-x}, \quad \frac{\partial v}{\partial y} = \frac{v}{y}, \quad \frac{\partial v}{\partial z} = \frac{-v}{z-x}$$

$$\frac{\partial w}{\partial x} = \frac{-w}{x-y}, \quad \frac{\partial w}{\partial y} = \frac{w}{x-y}, \quad \frac{\partial w}{\partial z} = \frac{w}{z}$$

$$\therefore \frac{\partial(u, v, w)}{\partial(x, y, z)} = \begin{vmatrix} \frac{\partial u}{\partial x} & \frac{\partial u}{\partial y} & \frac{\partial u}{\partial z} \\ \frac{\partial v}{\partial x} & \frac{\partial v}{\partial y} & \frac{\partial v}{\partial z} \\ \frac{\partial w}{\partial x} & \frac{\partial w}{\partial y} & \frac{\partial w}{\partial z} \end{vmatrix}$$

$$= \begin{vmatrix} \frac{u}{x} & \frac{-u}{y-z} & \frac{u}{y-z} \\ \frac{v}{z-x} & \frac{v}{y} & \frac{-v}{z-x} \\ \frac{-w}{x-y} & \frac{w}{x-y} & \frac{w}{z} \end{vmatrix}$$

Taking out u, v, w from R_1, R_2, R_3 respectively

$$= uvw \begin{vmatrix} \frac{1}{x} & \frac{-1}{y-z} & \frac{1}{y-z} \\ \frac{1}{z-x} & \frac{1}{y} & \frac{-1}{z-x} \\ \frac{-1}{x-y} & \frac{1}{x-y} & \frac{1}{z} \end{vmatrix}$$

Multiplying R_1, R_2, R_3 by $y-z, z-x, x-y$ respectively

$$= \frac{uvw}{(y-z)(z-x)(x-y)} \begin{vmatrix} \frac{y-z}{x} & -1 & 1 \\ 1 & \frac{z-x}{y} & -1 \\ -1 & 1 & \frac{x-y}{z} \end{vmatrix}$$

Multiplying C_1, C_2, C_3 by x, z respectively

$$= \frac{uvw}{xyz(y-z)(z-x)(x-y)} \begin{vmatrix} \frac{y-z}{x} & -y & z \\ x & \frac{z-x}{y} & -z \\ -x & 1 & \frac{x-y}{z} \end{vmatrix}$$

Operating $C_1 \rightarrow C_1 + C_2 + C_3$

$$= \frac{1}{(y-z)^2(z-x)^2(x-y)^2} \begin{vmatrix} 0 & -y & z \\ 0 & z-x & -z \\ 0 & y & x-y \end{vmatrix} = 0$$

$$\left[\because \frac{u}{x} = \frac{1}{y-z}, \frac{v}{y} = \frac{1}{z-x}, \frac{w}{z} = \frac{1}{x-y} \right]$$

EXERCISE 10.4

1. If $u = x^2 - 2y$, $v = x + y$, prove that $\frac{\partial(u, v)}{\partial(x, y)} = 2x + 2$.
2. (a) If $u = x(1 - y)$, $v = xy$; prove that $JJ' = 1$.

(b) Prove that $JJ' = 1$ if $x = uv, y = \frac{u}{v}$

[Hint. $u = vy \Rightarrow x = v^2y \therefore v = \sqrt{\frac{x}{y}}$ and $u = \sqrt{xy}$]

3. (a) In polar coordinates, $x = r \cos \theta, y = r \sin \theta$, show that $\frac{\partial(x, y)}{\partial(r, \theta)} = r$.

(b) If $x = r \cos \theta, y = r \sin \theta$, verify that $\frac{\partial(x, y)}{\partial(r, \theta)} \cdot \frac{\partial(r, \theta)}{\partial(x, y)} = 1$.

[Hint. $r = \sqrt{x^2 + y^2}, \theta = \tan^{-1} \frac{y}{x}$]

4. If $x = r \cos \theta, y = r \sin \theta, z = z$, evaluate $\frac{\partial(x, y, z)}{\partial(r, \theta, z)}$.

Note. Here (x, y, z) and (r, θ, z) are respectively the Cartesian and cylindrical coordinates of a point.

5. (a) If $y_1 = \frac{x_2 x_3}{x_1}, y_2 = \frac{x_3 x_1}{x_2}, y_3 = \frac{x_1 x_2}{x_3}$, show that $\frac{\partial(y_1, y_2, y_3)}{\partial(x_1, x_2, x_3)} = 4$.

(U.P.T.U. 2006)

(b) If $u = \frac{yz}{x}, v = \frac{zx}{y}, w = \frac{xy}{z}$, show that $\frac{\partial(x, y, z)}{\partial(u, v, w)} = \frac{1}{4}$.

6. If $u = \frac{y^2}{2x}, v = \frac{x^2 + y^2}{2x}$, find $\frac{\partial(u, v)}{\partial(x, y)}$.

10.11. TAYLOR'S THEOREM FOR A FUNCTION OF TWO VARIABLES

We know that by Taylor's theorem for a function $f(x)$ of single variable x ,

$$f(x+h) = f(x) + hf'(x) + \frac{h^2}{2!} f''(x) + \frac{h^3}{3!} f'''(x) + \dots$$

Now let $f(x, y)$ be a function of two independent variables x and y . If y is kept constant, then by Taylor's theorem for a function of a single variable x , we have

$$f(x+h, y+k) = f(x, y+k) + h \frac{\partial}{\partial x} f(x, y+k) + \frac{h^2}{2!} \cdot \frac{\partial^2}{\partial x^2} f(x, y+k) + \frac{h^3}{3!} \cdot \frac{\partial^3}{\partial x^3} f(x, y+k) + \dots \quad \dots(1)$$

Now keeping x constant and applying Taylor's theorem for a function of a single variable y , we have

$$f(x, y+k) = f(x, y) + k \frac{\partial}{\partial y} f(x, y) + \frac{k^2}{2!} \cdot \frac{\partial^2}{\partial y^2} f(x, y) + \frac{k^3}{3!} \cdot \frac{\partial^3}{\partial y^3} f(x, y) + \dots \quad \dots(2)$$

Using (2), we can write (1) as

$$\begin{aligned} f(x+h, y+k) = & \left[f(x, y) + k \frac{\partial}{\partial y} f(x, y) + \frac{k^2}{2!} \cdot \frac{\partial^2}{\partial y^2} f(x, y) + \frac{k^3}{3!} \cdot \frac{\partial^3}{\partial y^3} f(x, y) + \dots \right] \\ & + h \frac{\partial}{\partial x} \left[f(x, y) + k \frac{\partial}{\partial y} f(x, y) + \frac{k^2}{2!} \cdot \frac{\partial^2}{\partial y^2} f(x, y) + \dots \right] \\ & + \frac{h^2}{2!} \cdot \frac{\partial^2}{\partial x^2} \left[f(x, y) + k \frac{\partial}{\partial y} f(x, y) + \dots \right] + \frac{h^3}{3!} \cdot \frac{\partial^3}{\partial x^3} [f(x, y) + \dots] + \dots \end{aligned}$$

$$\begin{aligned}
&= \left[f(x, y) + h \frac{\partial f}{\partial y} + \frac{h^2}{2!} \cdot \frac{\partial^2 f}{\partial y^2} + \frac{h^3}{3!} \cdot \frac{\partial^3 f}{\partial y^3} + \dots \right] \\
&+ \left[h \frac{\partial f}{\partial x} + hk \frac{\partial^2 f}{\partial x \partial y} + \frac{hk^2}{2!} \cdot \frac{\partial^3 f}{\partial x \partial y^2} + \dots \right] \\
&+ \left[\frac{h^2}{2!} \cdot \frac{\partial^2 f}{\partial x^2} + \frac{h^2 k}{2!} \cdot \frac{\partial^3 f}{\partial x^2 \partial y} + \dots \right] \\
&+ \frac{h^3}{3!} \frac{\partial^3 f}{\partial x^3} + \dots \\
&= f(x, y) + \left(h \frac{\partial f}{\partial x} + k \frac{\partial f}{\partial y} \right) + \left(\frac{h^2}{2!} \cdot \frac{\partial^2 f}{\partial x^2} + hk \frac{\partial^2 f}{\partial x \partial y} + \frac{k^2}{2!} \cdot \frac{\partial^2 f}{\partial y^2} \right) \\
&\quad + \left(\frac{h^3}{3!} \cdot \frac{\partial^3 f}{\partial x^3} + \frac{h^2 k}{2!} \cdot \frac{\partial^3 f}{\partial x^2 \partial y} + \frac{hk^2}{2!} \cdot \frac{\partial^3 f}{\partial x \partial y^2} + \frac{k^3}{3!} \cdot \frac{\partial^3 f}{\partial y^3} \right) + \dots \\
&= f(x, y) + \left(h \frac{\partial f}{\partial x} + k \frac{\partial f}{\partial y} \right) + \frac{1}{2!} \left(h^2 \frac{\partial^2 f}{\partial x^2} + 2hk \frac{\partial^2 f}{\partial x \partial y} + k^2 \frac{\partial^2 f}{\partial y^2} \right) \\
&\quad + \frac{1}{3!} \left(h^3 \frac{\partial^3 f}{\partial x^3} + 3h^2 k \frac{\partial^3 f}{\partial x^2 \partial y} + 3hk^2 \frac{\partial^3 f}{\partial x \partial y^2} + k^3 \frac{\partial^3 f}{\partial y^3} \right) + \dots \\
&= f(x, y) + \left(h \frac{\partial}{\partial x} + k \frac{\partial}{\partial y} \right) f + \frac{1}{2!} \left(h \frac{\partial}{\partial x} + k \frac{\partial}{\partial y} \right)^2 f + \frac{1}{3!} \left(h \frac{\partial}{\partial x} + k \frac{\partial}{\partial y} \right)^3 f + \dots
\end{aligned}$$

Cor. 1. Putting $x = a$ and $y = b$, we have

$$\begin{aligned}
&f(a + h, b + k) + f(a, b) + [hf_x(a, b) + kf_y(a, b)] + \frac{1}{2!} [h^2 f_{xx}(a, b) + 2hk f_{xy}(a, b) + k^2 f_{yy}(a, b)] \\
&\quad + \frac{1}{3!} [h^3 f_{xxx}(a, b) + 3h^2 k f_{xxy}(a, b) + 3hk^2 f_{xyy}(a, b) + k^3 f_{yyy}(a, b)] + \dots
\end{aligned}$$

Cor. 2. In Cor. 1, putting $a + h = x$ and $b + k = y$ so that $h = x - a$ and $k = y - b$, we have

$$\begin{aligned}
f(x, y) = f(a, b) + [(x - a) f_x(a, b) + (y - b) f_y(a, b)] + \frac{1}{2!} [(x - a)^2 f_{xx}(a, b) + 2(x - a)(y - b) \\
f_{xy}(a, b) + (y - b)^2 f_{yy}(a, b)] + \dots
\end{aligned}$$

Cor. 3. Putting $a = 0, b = 0$ in Cor. 2, we have

$$f(x, y) = f(0, 0) + [xf_x(0, 0) + yf_y(0, 0)] + \frac{1}{2!} [x^2 f_{xx}(0, 0) + 2xy f_{xy}(0, 0) + y^2 f_{yy}(0, 0)] + \dots$$

This is called Maclaurin's theorem for two variables.

Note. Cor. 3 is used to expand $f(x, y)$ in powers of x and y [or to expand $f(x, y)$ in the neighbourhood of origin $(0, 0)$].

Cor. 2 is used to expand $f(x, y)$ in the neighbourhood of (a, b) .

ILLUSTRATIVE EXAMPLES

Example 1. Expand $e^x \sin y$ in powers of x and y as far as terms of the third degree.

Sol. Here $f(x, y) = e^x \sin y$; $f(0, 0) = 0$
 $f_x(x, y) = e^x \sin y$, $f_x(0, 0) = 0$
 $f_y(x, y) = e^x \cos y$, $f_y(0, 0) = 1$
 $f_{xx}(x, y) = e^x \sin y$, $f_{xx}(0, 0) = 0$
 $f_{xy}(x, y) = e^x \cos y$, $f_{xy}(0, 0) = 1$
 $f_{yy}(x, y) = -e^x \sin y$, $f_{yy}(0, 0) = 0$
 $f_{xxx}(x, y) = e^x \sin y$, $f_{xxx}(0, 0) = 0$
 $f_{xxy}(x, y) = e^x \cos y$, $f_{xxy}(0, 0) = 1$
 $f_{xyy}(x, y) = -e^x \sin y$, $f_{xyy}(0, 0) = 0$
 $f_{yyy}(x, y) = -e^x \cos y$, $f_{yyy}(0, 0) = -1$

$\therefore e^x \sin y = f(x, y)$

$$\begin{aligned}
 &= f(0, 0) + [xf_x(0, 0) + yf_y(0, 0)] + \frac{1}{2!} [x^2 f_{xx}(0, 0) + 2xy f_{xy}(0, 0) + y^2 f_{yy}(0, 0)] \\
 &\quad + \frac{1}{3!} [x^3 f_{xxx}(0, 0) + 3x^2 y f_{xxy}(0, 0) + 3xy^2 f_{xyy}(0, 0) + y^3 f_{yyy}(0, 0)] + \dots \\
 &= 0 + [x \cdot 0 + y \cdot 1] + \frac{1}{2!} [x^2 \cdot 0 + 2xy \cdot 1 + y^2 \cdot 0] + \frac{1}{3!} [x^3 \cdot 0 + 3x^2 y \cdot 1 + 3xy^2 \\
 &\quad + 0 + y^3(-1)] + \dots \\
 &= y + xy + \frac{1}{2} x^2 y - \frac{1}{6} y^3 + \dots
 \end{aligned}$$

Example 2. Expand $f(x, y) = \tan^{-1} \frac{y}{x}$ in powers of $(x - 1)$ and $(y - 1)$ upto third degree terms. Hence compute $f(1.1, 0.9)$ approximately.

(M.D.U. Dec. 2007 ; U.P.T.U. 2006 ; J.N.T.U. 2006)

Sol. Here $f(x, y) = \tan^{-1} \frac{y}{x}$, $f(1, 1) = \tan^{-1} 1 = \frac{\pi}{4}$

$$f_x(x, y) = \frac{1}{1 + \frac{y^2}{x^2}} \cdot \left(-\frac{y}{x^2} \right) = -\frac{y}{x^2 + y^2} , f_x(1, 1) = -\frac{1}{2}$$

$$f_y(x, y) = \frac{1}{1 + \frac{y^2}{x^2}} \cdot \frac{1}{x} = \frac{x}{x^2 + y^2} , f_y(1, 1) = \frac{1}{2}$$

$$f_{xx}(x, y) = -y(-1)(x^2 + y^2)^{-2} \cdot 2x = \frac{2xy}{(x^2 + y^2)^2} , f_{xx}(1, 1) = \frac{1}{2}$$

$$f_{xy}(x, y) = \frac{(x^2 + y^2) \cdot 1 - x \cdot 2x}{(x^2 + y^2)^2} = \frac{y^2 - x^2}{(x^2 + y^2)^2} , f_{xy}(1, 1) = 0$$

$$f_{yy}(x, y) = x(-1)(x^2 + y^2)^{-2} \cdot 2y = -\frac{2xy}{(x^2 + y^2)^2} , f_{yy}(1, 1) = -\frac{1}{2}$$

$$f_{xxx}(x, y) = 2y \cdot \frac{(x^2 + y^2)^2 \cdot 1 - x \cdot 2(x^2 + y^2) \cdot 2x}{(x^2 + y^2)^4} = 2y \cdot \frac{(x^2 + y^2) - 4x^2}{(x^2 + y^2)^3}$$

$$= \frac{2y(y^2 - 3x^2)}{(x^2 + y^2)^3}, \quad f_{xx}(1, 1) = -\frac{1}{2}$$

$$f_{xy}(x, y) = \frac{(x^2 + y^2)^2(-2x) - (y^2 - x^2) \cdot 2(x^2 + y^2) \cdot 2x}{(x^2 + y^2)^4}$$

$$= \frac{(x^2 + y^2)(-2x) - 4x(y^2 - x^2)}{(x^2 + y^2)^3} = \frac{2x(x^2 - 3y^2)}{(x^2 + y^2)^3}, \quad f_{xy}(1, 1) = -\frac{1}{2}$$

$$f_{yy}(x, y) = -2y \cdot \frac{(x^2 + y^2)^2 \cdot 1 - x \cdot 2(x^2 + y^2) \cdot 2x}{(x^2 + y^2)^4} = \frac{-2y(x^2 + y^2 - 4x^2)}{(x^2 + y^2)^3}$$

$$= \frac{2y(3x^2 - y^2)}{(x^2 + y^2)^3}, \quad f_{yy}(1, 1) = \frac{1}{2}$$

$$f_{yyy}(x, y) = -2x \cdot \frac{(x^2 + y^2)^2 \cdot 1 - y \cdot 2(x^2 + y^2) \cdot 2y}{(x^2 + y^2)^4} = \frac{-2x(x^2 + y^2 - 4y^2)}{(x^2 + y^2)^3}$$

$$= \frac{2x(3y^2 - x^2)}{(x^2 + y^2)^3}, \quad f_{yyy}(1, 1) = \frac{1}{2}$$

$$\therefore \tan^{-1} \frac{y}{x} = f(x, y) = f(1, 1) + [(x-1)f_x(1, 1) + (y-1)f_y(1, 1)]$$

$$+ \frac{1}{2!} [(x-1)^2 f_{xx}(1, 1) + 2(x-1)(y-1)f_{xy}(1, 1) + (y-1)^2 f_{yy}(1, 1)]$$

$$+ \frac{1}{3!} [(x-1)^3 f_{xxx}(1, 1) + 3(x-1)^2(y-1)f_{xxy}(1, 1)$$

$$+ 3(x-1)(y-1)^2 f_{xyy}(1, 1) + (y-1)^3 f_{yyy}(1, 1)] + \dots$$

$$= \frac{\pi}{4} + \left[(x-1)\left(-\frac{1}{2}\right) + (y-1)\left(\frac{1}{2}\right) \right] + \frac{1}{2} \left[(x-1)^2 \left(\frac{1}{2}\right) + 2(x-1)(y-1)(0) + (y-1)^2 \left(-\frac{1}{2}\right) \right]$$

$$+ \frac{1}{6} \left[(x-1)^3 \left(-\frac{1}{2}\right) + 3(x-1)^2(y-1)\left(-\frac{1}{2}\right) + 3(x-1)(y-1)^2 \left(\frac{1}{2}\right) + (y-1)^3 \left(\frac{1}{2}\right) \right] + \dots$$

$$= \frac{\pi}{4} - \frac{1}{2} [(x-1) - (y-1)] + \frac{1}{4} [(x-1)^2 - (y-1)^2] - \frac{1}{12} [(x-1)^3$$

$$+ 3(x-1)^2(y-1) - 3(x-1)(y-1)^2 - (y-1)^3] + \dots$$

Putting $x = 1.1$ and $y = 0.9$, we get

$$f(1.1, 0.9) = \frac{\pi}{4} - \frac{1}{2}(0.2) + \frac{1}{4}(0) - \frac{1}{12} [(0.1)^3 + 3(0.1)^2(-0.1) - 3(0.1)(-0.1)^2 - (-0.1)^3]$$

$$= 0.7854 - 0.1 + 0.0003 = 0.6857.$$

Example 3. Expand $e^x \log(1+y)$ in powers of x and y upto terms of third degree.
(J.N.T.U. 2006 ; M.D.U. May 2008 ; P.T.U. 2006)

Sol. Here

$$f(x, y) = e^x \log(1+y),$$

$$f_x(x, y) = e^x \log(1+y).$$

$$f_y(x, y) = \frac{e^x}{1+y},$$

$$f_{xx}(x, y) = e^x \log(1+y),$$

$$f_{xy}(x, y) = \frac{e^x}{1+y},$$

$$f(0, 0) = 0$$

$$f_x(0, 0) = 0$$

$$f_y(0, 0) = 1$$

$$f_{xx}(0, 0) = 0$$

$$f_{xy}(0, 0) = 1$$

$$\begin{aligned}
 f_{yy}(x, y) &= -\frac{e^x}{(1+y)^2}, & f_{yy}(0, 0) &= -1 \\
 f_{xxx}(x, y) &= e^x \log(1+y), & f_{xxx}(0, 0) &= 0 \\
 f_{xy}(x, y) &= \frac{e^x}{1+y}, & f_{xy}(0, 0) &= 1 \\
 f_{xyy}(x, y) &= -\frac{e^x}{(1+y)^2}, & f_{xyy}(0, 0) &= -1 \\
 f_{yyy}(x, y) &= \frac{2e^x}{(1+y)^3}, & f_{yyy}(0, 0) &= 2
 \end{aligned}$$

$$\therefore e^x \log(1+y) = f(x, y)$$

$$\begin{aligned}
 &= f(0, 0) + [xf_x(0, 0) + yf_y(0, 0)] + \frac{1}{2!} [x^2 f_{xx}(0, 0) + 2xy f_{xy}(0, 0) + y^2 f_{yy}(0, 0)] \\
 &\quad + \frac{1}{3!} [x^3 f_{xxx}(0, 0) + 3x^2 y f_{xxy}(0, 0) + 3xy^2 f_{xyy}(0, 0) + y^3 f_{yyy}(0, 0)] + \dots \\
 &= 0 + [x \cdot 0 + y \cdot 1] + \frac{1}{2} [x^2 \cdot 0 + 2xy \cdot 1 + y^2 \cdot (-1)] + \frac{1}{6} [x^3 \cdot 0 + 3x^2 y \cdot 1 + 3xy^2 \cdot (-1) + y^3 \cdot 2] + \dots \\
 &= y + xy - \frac{1}{2}y^2 + \frac{1}{2}x^2y - \frac{1}{2}xy^2 + \frac{1}{3}y^3 \dots
 \end{aligned}$$

Example 4. Expand $\frac{(x+h)(y+k)}{x+h+y+k}$ in powers of h, k upto and inclusive of the second degree terms.

Sol. Here $f(x+h, y+k) = \frac{(x+h)(y+k)}{x+h+y+k}$

Putting $h = k = 0$, we have $f(x, y) = \frac{xy}{x+y}$

$$f_x = \frac{(x+y) \cdot y - xy \cdot 1}{(x+y)^2} = \frac{y^2}{(x+y)^2}; \quad f_y = \frac{x^2}{(x+y)^2}, \text{ by symmetry}$$

$$f_{xx} = -\frac{2y^2}{(x+y)^3}, \quad f_{yy} = -\frac{2x^2}{(x+y)^3}$$

$$f_{xy} = \frac{(x+y)^2 \cdot 2x - x^2 \cdot 2(x+y)}{(x+y)^4} = \frac{2x(x+y) - 2x^2}{(x+y)^3} = \frac{2xy}{(x+y)^3}$$

$$\begin{aligned}
 \therefore \frac{(x+h)(y+k)}{x+h+y+k} &= f(x+h, y+k) = f(x, y) + [hf_x + kf_y] + \frac{1}{2!} [h^2 f_{xx} + 2hk f_{xy} + k^2 f_{yy}] + \dots \\
 &= \frac{xy}{x+y} + \left[h \cdot \frac{y^2}{(x+y)^2} + k \cdot \frac{x^2}{(x+y)^2} \right] \\
 &\quad + \frac{1}{2} \left[h^2 \cdot \frac{-2y^2}{(x+y)^3} + 2hk \cdot \frac{2xy}{(x+y)^3} + k^2 \cdot \frac{-2x^2}{(x+y)^3} \right] + \dots \\
 &= \frac{xy}{x+y} + \frac{y^2}{(x+y)^2} \cdot h + \frac{x^2}{(x+y)^2} \cdot k - \frac{y^2}{(x+y)^3} \cdot h^2 \\
 &\quad + \frac{2xy}{(x+y)^3} \cdot hk - \frac{x^2}{(x+y)^3} \cdot k^2 + \dots
 \end{aligned}$$

Example 5. Expand $x^2y + 3y - 2$ in powers of $(x - 1)$ and $(y + 2)$ using Taylor's Theorem.
(M.D.U. May 2006, Dec. 2006 ; U.P.T.U. 2006 ; Anna 2005)

Sol. Expansion of $f(x, y)$ in powers of $(x - a)$ and $(y - b)$ is given by

$$\begin{aligned} f(x, y) = & f(a, b) + [(x - a)f_x(a, b) + (y - b)f_y(a, b)] + \frac{1}{2!} [(x - a)^2 f_{xx}(a, b) \\ & + 2(x - a)(y - b)f_{xy}(a, b) + (y - b)^2 f_{yy}(a, b)] + \frac{1}{3!} [(x - a)^3 f_{xxx}(a, b) \\ & + 3(x - a)^2(y - b)f_{xxy}(a, b) + 3(x - a)(y - b)^2 f_{xyy}(a, b) + (y - b)^3 f_{yyy}(a, b)] \\ & + \dots \end{aligned} \quad \dots(1)$$

Here $f(x, y) = x^2y + 3y - 2$, $a = 1$, $b = -2$

$$f(1, -2) = 1^2 \times (-2) + 3(-2) - 2 = -10$$

$$\begin{aligned} f_x &= 2xy, & f_x(1, -2) &= 2(1)(-2) = -4; & f_y &= x^2 + 3, & f_y(1, -2) &= 1^2 + 3 = 4 \\ f_{xx} &= 2y, & f_{xx}(1, -2) &= 2(-2) = -4; & f_{xy} &= 2x, & f_{xy}(1, -2) &= 2(1) = 2 \\ f_{yy} &= 0, & f_{yy}(1, -2) &= 0; & f_{xxx} &= 0, & f_{xxx}(1, -2) &= 0 \\ f_{xxy} &= 2, & f_{xxy}(1, -2) &= 2; & f_{xyy} &= 0, & f_{xyy}(1, -2) &= 0 \\ f_{yyy} &= 0, & f_{yyy}(1, -2) &= 0 \end{aligned}$$

All higher order partial derivatives vanish.

\therefore From (1), we have

$$x^2y + 3y - 2 = f(x, y)$$

$$\begin{aligned} &= -10 + [(x - 1)(-4) + (y + 2)(4)] + \frac{1}{2} [(x - 1)^2(-4) + 2(x - 1)(y + 2)(2) + (y + 2)^2(0)] \\ &\quad + \frac{1}{6} [(x - 1)^3(0) + 3(x - 1)^2(y + 2)(2) + 3(x - 1)(y + 2)^2(0) + (y + 2)^3(0)] \\ &= -10 - 4(x - 1) + 4(y + 2) - 2(x - 1)^2 + 2(x - 1)(y + 2) + (x - 1)^2(y + 2). \end{aligned}$$

EXERCISE 10.5

1. Show that $e^y \log(1 + x) = x + xy - \frac{x^2}{2}$ approximately.

[Hint. Find the expansion at $(0, 0)$]

2. Expand $e^x \cos y$ in powers of x and y as far as the terms of third degree.
3. Expand $e^{ax} \sin by$ in powers of x and y as far as the terms of third degree. (M.D.U. May 2005)
4. Expand e^{xy} at $(1, 1)$ in powers of $(x - 1)$ and $(y - 1)$.
5. Expand $e^x \cos y$ about $\left(1, \frac{\pi}{4}\right)$.
6. Expand $e^x \cos y$ about $\left(1, \frac{\pi}{4}\right)$.